top_down and bottom_up rewriting.

theories/Lambda/AutoSetoidRewrite2.v
@@ -1,3 +1,4 @@
+Require Import Coq.Classes.Morphisms.
 Require Import Coq.PArith.BinPos.
 Require Import Coq.Relations.Relations.
 Require Import Coq.FSets.FMapPositive.
@@ -8,6 +9,7 @@ Require Import ExtLib.Recur.GenRec.
 Require Import ExtLib.Tactics.
 Require Import MirrorCore.Lambda.Expr.
 Require Import MirrorCore.Lambda.ExprTac.
+Require Import MirrorCore.Lambda.AppN.
 
 Set Implicit Arguments.
 Set Strict Implicit.
@@ -37,52 +39,6 @@ Section setoid.
   | Rrespects (l r : R)
   | Rpointwise (t : typ) (r : R).
 
-  Definition mrw (T : Type) : Type :=
-    option T.
-  Definition rw_ret {T} (val : T) : mrw T :=
-    Some val.
-  Definition rw_bind {T U} (c : mrw T) (k : T -> mrw U) : mrw U :=
-    match c with
-      | None => None
-      | Some v => k v
-    end.
-  Definition rw_orelse {T} (c1 c2 : mrw T) : mrw T :=
-    match c1 with
-      | None => c2
-      | z => z
-    end.
-  Definition rw_fail {T} : mrw T := None.
-
-  Let rewrite_expr :=
-    forall (es : list (expr typ func * (R -> mrw (expr typ func))))
-           (rg : R),
-      mrw (expr typ func).
-  Variable respectfulness
-  : expr typ func -> rewrite_expr.
-
-  Fixpoint setoid_rewrite2 (e : expr typ func)
-           (es : list (expr typ func * (R -> mrw (expr typ func)))) (rg : R)
-  : mrw (expr typ func) :=
-    match e with
-      | App f x =>
-        setoid_rewrite2 f ((x, setoid_rewrite2 x nil) :: es) rg
-      | Abs t e' =>
-        match es with
-          | nil => match rg with
-                     | Rpointwise _t (*=t*) rg' =>
-                       rw_bind (setoid_rewrite2 e' nil rg')
-                               (fun e'' => rw_ret (Abs t e''))
-                     | _ => respectfulness (Abs t e') es rg
-                   end
-          | _ => respectfulness (Abs t e') es rg
-        end
-      | Var v => respectfulness (Var v) es rg
-      | UVar u => respectfulness (UVar u) es rg
-      | Inj i => respectfulness (Inj i) es rg
-    end.
-
-  Require Import Coq.Classes.Morphisms.
-
   Variable RbaseD : Rbase -> forall t : typ, option (relation (typD t)).
   Fixpoint RD (r : R) (t : typ) : option (relation (typD t)) :=
     match r with
@@ -109,90 +65,203 @@ Section setoid.
                    None
     end.
 
-  Require Import MirrorCore.Lambda.AppN.
 
-  Definition setoid_rewrite2_rec tus tvs (ls : list (expr typ func * (R -> mrw (expr typ func)))) : Prop :=
-    Forall (fun e =>
-              forall t eD,
-                exprD' tus tvs t (fst e) = Some eD ->
-                forall r e' rD,
-                  snd e r = Some e' ->
-                  RD r t = Some rD ->
-                  exists eD',
-                    exprD' tus tvs t e' = Some eD' /\
-                    forall us vs,
-                      rD (eD us vs) (eD' us vs)) ls.
+  Definition mrw (T : Type) : Type :=
+    option T.
+  Definition rw_ret {T} (val : T) : mrw T :=
+    Some val.
+  Definition rw_bind {T U} (c : mrw T) (k : T -> mrw U) : mrw U :=
+    match c with
+      | None => None
+      | Some v => k v
+    end.
+  Definition rw_orelse {T} (c1 c2 : mrw T) : mrw T :=
+    match c1 with
+      | None => c2
+      | z => z
+    end.
+  Definition rw_fail {T} : mrw T := None.
 
-  Hypothesis respectfulness_sound
-  : forall e e' tus tvs t es rg rD eesD,
-      respectfulness e es rg = Some e' ->
-      RD rg t = Some rD ->
-      exprD' tus tvs t (apps e (map fst es)) = Some eesD ->
-      setoid_rewrite2_rec tus tvs es ->
-      exists eesD',
-        exprD' tus tvs t e' = Some eesD' /\
-        forall us vs,
-          rD (eesD us vs) (eesD' us vs).
+  Section rw_map2.
+    Context {T U V : Type}.
+    Variable f : T -> U -> mrw V.
 
-  Theorem setoid_rewrite2_sound
-  : forall e e' tus tvs t es rg rD eesD,
-      setoid_rewrite2 e es rg = Some e' ->
-      RD rg t = Some rD ->
-      exprD' tus tvs t (apps e (map fst es)) = Some eesD ->
-      setoid_rewrite2_rec tus tvs es ->
-      exists eesD',
-        exprD' tus tvs t e' = Some eesD' /\
-        forall us vs,
-          rD (eesD us vs) (eesD' us vs).
-  Proof.
-    induction e; simpl; intros; eauto using respectfulness_sound.
-    { (* App *)
-      eapply IHe1 in H; eauto.
-      constructor; eauto.
-      simpl. intros. eapply IHe2; eauto. constructor. }
-    { (* Abs *)
-      destruct es; eauto.
-      destruct rg; eauto.
-      unfold rw_bind in H.
-      consider (setoid_rewrite2 e nil rg).
-      - intros. inversion H3; clear H3; subst.
-        rewrite exprD'_apps in H1; eauto. simpl in H1.
-        unfold apps_sem' in H1.
-        simpl in H1.
-        { consider (typeof_expr tus (t :: tvs) e); intros.
-          - consider (exprD' tus tvs (typ2 t t2) (Abs t e)); intros.
-            + consider (type_cast (typ2 t t2) t0); intros.
-              * inv_all. subst.
-                revert H3.
-                autorewrite with exprD_rw. simpl.
-                destruct r.
-                repeat rewrite typ2_match_zeta; eauto.
-                repeat rewrite type_cast_refl; eauto.
-                consider (exprD' tus (t :: tvs) t2 e); intros.
-                { autorewrite with eq_rw in H5.
-                  inv_all; subst.
-                  simpl in H0. rewrite typ2_match_zeta in H0; eauto.
-                  consider (type_cast (typ2 t t2) t1); intros.
-                  - generalize dependent (typ2_cast t t2).
-                    intro e1. autorewrite with eq_rw.
-                    consider (RD rg t2); intros.
-                    + inv_all; subst.
-                      eapply IHe in H; eauto.
-                      2: constructor.
-                      forward_reason.
-                      change_rewrite H.
-                      eexists; split; eauto.
-                      destruct r. unfold Rcast. simpl.
-                      unfold relation. intros. autorewrite with eq_rw.
-                      red. intros. eapply H6.
-                    + inversion H6.
-                  - clear - H5. autorewrite with eq_rw in H5. inversion H5. }
-                { autorewrite with eq_rw in H5. inversion H5. }
-              * inversion H5.
-            + inversion H4.
-          - inversion H3. }
-      - inversion 2. }
-  Qed.
+    Fixpoint rw_map2 (ts : list T) (us : list U) : mrw (list V) :=
+      match ts , us with
+        | nil , nil => rw_ret nil
+        | t :: ts , u :: us =>
+          rw_bind (f t u) (fun v =>
+                             rw_bind (rw_map2 ts us)
+                                     (fun vs => rw_ret (v :: vs)))
+        | _ , _ => rw_fail
+      end.
+  End rw_map2.
+
+
+  Let rewrite_expr :=
+    forall (es : list (expr typ func * (R -> mrw (expr typ func))))
+           (rg : R),
+      mrw (expr typ func).
+  Section setoid_rewrite.
+    Variable respectfulness
+    : expr typ func -> rewrite_expr.
+
+
+    Fixpoint setoid_rewrite2 (e : expr typ func)
+             (es : list (expr typ func * (R -> mrw (expr typ func)))) (rg : R)
+    : mrw (expr typ func) :=
+      match e with
+        | App f x =>
+          setoid_rewrite2 f ((x, setoid_rewrite2 x nil) :: es) rg
+        | Abs t e' =>
+          match es with
+            | nil => match rg with
+                       | Rpointwise _t (*=t*) rg' =>
+                         rw_bind (setoid_rewrite2 e' nil rg')
+                                 (fun e'' => rw_ret (Abs t e''))
+                       | _ => respectfulness (Abs t e') es rg
+                     end
+            | _ => respectfulness (Abs t e') es rg
+          end
+        | Var v => respectfulness (Var v) es rg
+        | UVar u => respectfulness (UVar u) es rg
+        | Inj i => respectfulness (Inj i) es rg
+      end.
+
+    Definition setoid_rewrite2_rec tus tvs (ls : list (expr typ func * (R -> mrw (expr typ func)))) : Prop :=
+      Forall (fun e =>
+                forall t eD,
+                  exprD' tus tvs t (fst e) = Some eD ->
+                  forall r e' rD,
+                    snd e r = Some e' ->
+                    RD r t = Some rD ->
+                    exists eD',
+                      exprD' tus tvs t e' = Some eD' /\
+                      forall us vs,
+                        rD (eD us vs) (eD' us vs)) ls.
+
+    Hypothesis respectfulness_sound
+    : forall e e' tus tvs t es rg rD eesD,
+        respectfulness e es rg = Some e' ->
+        RD rg t = Some rD ->
+        exprD' tus tvs t (apps e (map fst es)) = Some eesD ->
+        setoid_rewrite2_rec tus tvs es ->
+        exists eesD',
+          exprD' tus tvs t e' = Some eesD' /\
+          forall us vs,
+            rD (eesD us vs) (eesD' us vs).
+
+    Theorem setoid_rewrite2_sound
+    : forall e e' tus tvs t es rg rD eesD,
+        setoid_rewrite2 e es rg = Some e' ->
+        RD rg t = Some rD ->
+        exprD' tus tvs t (apps e (map fst es)) = Some eesD ->
+        setoid_rewrite2_rec tus tvs es ->
+        exists eesD',
+          exprD' tus tvs t e' = Some eesD' /\
+          forall us vs,
+            rD (eesD us vs) (eesD' us vs).
+    Proof.
+      induction e; simpl; intros; eauto using respectfulness_sound.
+      { (* App *)
+        eapply IHe1 in H; eauto.
+        constructor; eauto.
+        simpl. intros. eapply IHe2; eauto. constructor. }
+      { (* Abs *)
+        destruct es; eauto.
+        destruct rg; eauto.
+        unfold rw_bind in H.
+        consider (setoid_rewrite2 e nil rg).
+        - intros. inversion H3; clear H3; subst.
+          rewrite exprD'_apps in H1; eauto. simpl in H1.
+          unfold apps_sem' in H1.
+          simpl in H1.
+          { consider (typeof_expr tus (t :: tvs) e); intros.
+            - consider (exprD' tus tvs (typ2 t t2) (Abs t e)); intros.
+              + consider (type_cast (typ2 t t2) t0); intros.
+                * inv_all. subst.
+                  revert H3.
+                  autorewrite with exprD_rw. simpl.
+                  destruct r.
+                  repeat rewrite typ2_match_zeta; eauto.
+                  repeat rewrite type_cast_refl; eauto.
+                  consider (exprD' tus (t :: tvs) t2 e); intros.
+                  { autorewrite with eq_rw in H5.
+                    inv_all; subst.
+                    simpl in H0. rewrite typ2_match_zeta in H0; eauto.
+                    consider (type_cast (typ2 t t2) t1); intros.
+                    - generalize dependent (typ2_cast t t2).
+                      intro e1. autorewrite with eq_rw.
+                      consider (RD rg t2); intros.
+                      + inv_all; subst.
+                        eapply IHe in H; eauto.
+                        2: constructor.
+                        forward_reason.
+                        change_rewrite H.
+                        eexists; split; eauto.
+                        destruct r. unfold Rcast. simpl.
+                        unfold relation. intros. autorewrite with eq_rw.
+                        red. intros. eapply H6.
+                      + inversion H6.
+                    - clear - H5. autorewrite with eq_rw in H5. inversion H5. }
+                  { autorewrite with eq_rw in H5. inversion H5. }
+                * inversion H5.
+              + inversion H4.
+            - inversion H3. }
+        - inversion 2. }
+    Qed.
+  End setoid_rewrite.
+
+  Section bottom_up.
+    Context (reflexive transitive : R -> bool)
+            (rw : expr typ func -> R -> option (expr typ func))
+            (respectful : expr typ func -> list (expr typ func) -> R -> option (list R)).
+
+    Definition bottom_up (e : expr typ func) (r : R) : option (expr typ func) :=
+      setoid_rewrite2
+        (fun e efs r =>
+	   let es := map fst efs in
+           rw_orelse
+	     match respectful e es r with
+	       | None => rw (apps e es) r
+	       | Some rs =>
+		 rw_bind (rw_map2 (fun f r => (snd f) r) efs rs)
+			 (fun es' => rw_ret (apps e es'))
+	     end
+	     (if reflexive r then rw_ret (apps e es) else rw_fail))
+        e nil r.
+  End bottom_up.
+
+  Section top_down.
+    Context (reflexive transitive : R -> bool)
+            (rw : expr typ func -> R -> option (expr typ func))
+            (respectful : expr typ func -> list (expr typ func) -> R -> option (list R)).
+
+    Fixpoint top_down (f : nat) (e : expr typ func) (r : R) {struct f}
+    : option (expr typ func) :=
+      setoid_rewrite2
+        (fun e efs r =>
+	   let es := map fst efs in
+           rw_orelse
+             (rw_bind (rw (apps e es) r)
+                      (fun e' =>
+                         if transitive r then
+                           match f with
+                             | 0 => rw_ret e'
+                             | S f => top_down f e' r
+                           end
+                         else
+                           rw_ret e'))
+             match respectful e es r with
+	       | None => if reflexive r then rw_ret (apps e es) else rw_fail
+	       | Some rs =>
+	         rw_orelse
+                   (rw_bind (rw_map2 (fun f r => (snd f) r) efs rs)
+		            (fun es' => rw_ret (apps e es')))
+                   (if reflexive r then rw_ret (apps e es) else rw_fail)
+	     end)
+        e nil r.
+  End top_down.
 
 End setoid.
 
